mechanization/theories/Core/Soundness/FunctionCases.v
@@ -9,8 +9,8 @@ From McPTS.Core.Soundness Require Import
   SortCases.
 Import Domain_Notations.
 
-Lemma cons_glu_sub_pred_pi_helper {P} (pred_P : PredicativeSig P) (full_P : FullSig P) : forall {sts Γ Sb Γ' σ ρ A a typ_rel exp_rel Γ'' τ M c s},
-    {{ EG Γ ∈ glu_ctx_env pred_P sts ↘ Sb }} ->
+Lemma cons_glu_sub_pred_pi_helper {P} (pred_P : PredicativeSig P) (full_P : FullSig P) : forall {Γ Sb Γ' σ ρ A a typ_rel exp_rel Γ'' τ M c s},
+    {{ EG Γ ∈ glu_ctx_env pred_P ↘ Sb }} ->
     {{ Γ' ⊢s σ ® ρ ∈ Sb }} ->
     {{ Γ ⊢ A : Sort@s }} ->
     {{ ⟦ A ⟧ ρ ↘ a }} ->
@@ -30,20 +30,20 @@ Qed.
 (* #[local] *)
 Hint Resolve cons_glu_sub_pred_pi_helper : mcpts.
 
-Lemma glu_rel_exp_pi {P} (pred_P : PredicativeSig P) (full_P : FullSig P) : forall {sts Γ A B s1 s2 s3 s1' s2' s3'} {r : Ru P s1 s2 s3},
+Lemma glu_rel_exp_pi {P} (pred_P : PredicativeSig P) (full_P : FullSig P) : forall {Γ A B s1 s2 s3 s1' s2' s3'} {r : Ru P s1 s2 s3},
     Ax P s3 s3' ->
-    {{ ⟪ pred_P ⟫ Γ : sts ⊩ A : Sort@s1 : s1'}} ->
-    {{ ⟪ pred_P ⟫ Γ, A : (s1 :: sts) ⊩ B : Sort@s2 : s2' }} ->
-    {{ ⟪ pred_P ⟫ Γ : sts ⊩ Π r A B : Sort@s3 : s3' }}.
+    {{ ⟪ pred_P ⟫ Γ ⊩ A : Sort@s1 > s1'}} ->
+    {{ ⟪ pred_P ⟫ Γ, A:Sort@s1 ⊩ B : Sort@s2 > s2' }} ->
+    {{ ⟪ pred_P ⟫ Γ ⊩ Π r A B : Sort@s3 > s3' }}.
 Proof.
   intros * Hax HA HB.
-  assert {{ ⟪ pred_P ⟫ ⊩ Γ : sts }} as [SbΓ] by mauto.
+  assert {{ ⟪ pred_P ⟫ ⊩ Γ }} as [SbΓ] by mauto.
   assert {{ Γ ⊢ A : Sort@s1 }} by mauto.
   inversion_clear HA as [SbΓ' []].
   handle_functional_glu_ctx_env P.
   rename SbΓ' into SbΓ.
-  assert {{ EG Γ, A ∈ glu_ctx_env pred_P (s1 :: sts) ↘ cons_glu_sub_pred pred_P s1 Γ A SbΓ }} by (econstructor; mauto; reflexivity).
-  assert {{ Γ, A ⊢ B : Sort@s2 }} by mauto.
+  assert {{ EG Γ, A:Sort@s1 ∈ glu_ctx_env pred_P ↘ cons_glu_sub_pred pred_P s1 Γ A SbΓ }} by (econstructor; mauto; reflexivity).
+  assert {{ Γ, A:Sort@s1 ⊢ B : Sort@s2 }} by mauto.
   inversion_clear HB as [SbΓA []].
   eapply glu_rel_exp_of_typ; mauto 3.
   intros.
@@ -60,7 +60,7 @@ Proof.
   destruct_conjs.
   rename m into a.
   assert {{ ⟪ pred_P ⟫ Γ ⊨u Π r A B : Sort@s3 }} as [env_relΓ]%rel_exp_unsorted_of_typ_inversion1 by mauto 3 using completeness_fundamental_exp.
-  assert {{ ⟪ pred_P ⟫ Γ, A ⊨u B : Sort@s2 }} as [env_relΓA]%rel_exp_unsorted_of_typ_inversion1 by mauto 3 using completeness_fundamental_exp.
+  assert {{ ⟪ pred_P ⟫ Γ, A:Sort@s1 ⊨u B : Sort@s2 }} as [env_relΓA]%rel_exp_unsorted_of_typ_inversion1 by mauto 3 using completeness_fundamental_exp.
   destruct_conjs.
   match_by_head1 (per_ctx_env pred_P env_relΓA) invert_per_ctx_env.
   pose env_relΓA.
@@ -70,24 +70,26 @@ Proof.
   eexists; repeat split; mauto.
   intros.
   match_by_head1 (@glu_sort_elem P) ltac:(fun H => directed invert_glu_sort_elem H).
-  assert (glu_sort_elem pred_P s1 IP IEL a).
-  {
-    assert ((pred_rel pred_P s1 s3 \/ s1 = s3) /\ (pred_rel pred_P s2 s3 \/ s2 = s3)) as [pr1 pr2] by (eapply ord_ru; mauto 2).
-    destruct glu_a as [glu_a_eq glu_a_rel].
-    destruct pr1;
-      [eapply glu_a_rel | subst; eapply glu_a_eq]; mauto 2.    
-  }
-  assert (forall c (equiv_c : in_rel c c) b,
-             {{ ⟦ B ⟧ ρ ↦ c ↘ b }} ->
-             glu_sort_elem pred_P s2 (OP c equiv_c) (OEL c equiv_c) b).
-  {
-    assert ((pred_rel pred_P s1 s3 \/ s1 = s3) /\ (pred_rel pred_P s2 s3 \/ s2 = s3)) as [pr1 pr2] by (eapply ord_ru; mauto 2).
-    intros.
-    assert ((s2 = s3 -> glu_sort_elem pred_P s3 (OP c equiv_c) (OEL c equiv_c) b) /\
-              (pred_rel pred_P s2 s3 -> glu_sort_elem pred_P s2 (OP c equiv_c) (OEL c equiv_c) b)) as [glu_b_eq glu_b_rel] by mauto 2.
-    destruct pr2;
-      [eapply glu_b_rel | subst; eapply glu_b_eq]; mauto 2.
-  }
+  rename x into OP, x0 into OEL.
+  rename H11 into IP, H13 into IEL.
+  (* assert (glu_sort_elem pred_P s1 IP IEL a). *)
+  (* { *)
+  (*   assert ((pred_rel pred_P s1 s3 \/ s1 = s3) /\ (pred_rel pred_P s2 s3 \/ s2 = s3)) as [pr1 pr2] by (eapply ord_ru; mauto 2). *)
+  (*   destruct glu_a as [glu_a_eq glu_a_rel]. *)
+  (*   destruct pr1; *)
+  (*     [eapply glu_a_rel | subst; eapply glu_a_eq]; mauto 2.     *)
+  (* } *)
+  (* assert (forall c (equiv_c : in_rel c c) b, *)
+  (*            {{ ⟦ B ⟧ ρ ↦ c ↘ b }} -> *)
+  (*            glu_sort_elem pred_P s2 (OP c equiv_c) (OEL c equiv_c) b). *)
+  (* { *)
+  (*   assert ((pred_rel pred_P s1 s3 \/ s1 = s3) /\ (pred_rel pred_P s2 s3 \/ s2 = s3)) as [pr1 pr2] by (eapply ord_ru; mauto 2). *)
+  (*   intros. *)
+  (*   assert ((s2 = s3 -> glu_sort_elem pred_P s3 (OP c equiv_c) (OEL c equiv_c) b) /\ *)
+  (*             (pred_rel pred_P s2 s3 -> glu_sort_elem pred_P s2 (OP c equiv_c) (OEL c equiv_c) b)) as [glu_b_eq glu_b_rel] by mauto 2. *)
+  (*   destruct pr2; *)
+  (*     [eapply glu_b_rel | subst; eapply glu_b_eq]; mauto 2. *)
+  (* } *)
   
   assert (per_sort_elem pred_P s1 (head_rel ρ ρ H21) a a) by mauto 2.
   handle_per_sort_elem_irrel.
@@ -112,16 +114,16 @@ Proof.
     assert {{ Δ' ⊢ B[σ∘τ,,M] ≈ B[q σ][τ,,M] : Sort@s2 }} as <-.
     {
       gen_presups.
-      assert {{ Δ' ⊢s q σ ∘ (τ ,, M) ≈ σ ∘ τ ,, M : Γ, A }} by (eapply sub_decompose_q; mauto 2).
+      assert {{ Δ' ⊢s q σ ∘ (τ ,, M) ≈ σ ∘ τ ,, M : Γ, A:Sort@s1 }} by (eapply sub_decompose_q; mauto 2).
       transitivity {{{ B[(q σ)∘(τ,,M)] }}}.
-      - eapply eq_exp_eq_sub_typ; mauto 3.
+      - eapply wf_exp_eq_sub_cong_sort; mauto 3.
       - eapply exp_eq_sub_compose_typ_sort; mauto 3.
         + eapply sub_q; mauto 2.
         + econstructor; mauto 2.
     }
     assert {{ Δ' ⊢s (σ∘τ),,M ® ρ ↦ m ∈ cons_glu_sub_pred pred_P s1 Γ A SbΓ }} as Hconspred by mauto 2.
     handle_functional_glu_ctx_env P.
-    assert (SbΓA Δ' {{{ σ∘τ,,M }}} d{{{ ρ ↦ m }}}) as Hconspred' by (eapply H35; eassumption).
+    assert (SbΓA Δ' {{{ σ∘τ,,M }}} d{{{ ρ ↦ m }}}) as Hconspred' by (eapply H30; eassumption).
     (on_all_hyp: fun H => destruct (H _ _ _ Hconspred')).
     simplify_evals.
     match_by_head (@glu_sort_elem P) ltac:(fun H => directed invert_glu_sort_elem H).
@@ -136,8 +138,8 @@ Qed.
 #[export]
 Hint Resolve glu_rel_exp_pi : mcpts.
 
-Lemma glu_rel_exp_of_pi {P} (pred_P : PredicativeSig P) (full_P : FullSig P) : forall {sts Γ M A B Sb s1 s2 s3} {r : Ru P s1 s2 s3},
-    {{ EG Γ ∈ glu_ctx_env pred_P sts ↘ Sb }} ->
+Lemma glu_rel_exp_of_pi {P} (pred_P : PredicativeSig P) (full_P : FullSig P) : forall {Γ M A B Sb s1 s2 s3} {r : Ru P s1 s2 s3},
+    {{ EG Γ ∈ glu_ctx_env pred_P ↘ Sb }} ->
     {{ ⟪ pred_P ⟫ Γ ⊨u Π r A B : Sort@s3 }} ->
     (forall Δ σ ρ,
         {{ Δ ⊢s σ ® ρ ∈ Sb }} ->
@@ -145,7 +147,7 @@ Lemma glu_rel_exp_of_pi {P} (pred_P : PredicativeSig P) (full_P : FullSig P) : f
           {{ ⟦ A ⟧ ρ ↘ a }} /\
             {{ ⟦ M ⟧ ρ ↘ m }} /\
             forall (typ_rel : glu_typ_pred P) (exp_rel : glu_exp_pred P), {{ DG Π r a ρ B ∈ glu_sort_elem pred_P s3 ↘ typ_rel ↘ exp_rel }} -> {{ Δ ⊢ M[σ] : (Π r A B)[σ] ® m ∈ exp_rel }}) ->
-    {{ ⟪ pred_P ⟫ Γ : sts ⊩ M : Π r A B : s3 }}.
+    {{ ⟪ pred_P ⟫ Γ ⊩ M : Π r A B > s3 }}.
 Proof.
   intros * ? [env_relΓ] Hbody.
   destruct_conjs.
@@ -176,26 +178,26 @@ Proof.
     eapply H5; mauto 2.
 Qed.
 
-Lemma glu_rel_exp_fn_helper {P} (pred_P : PredicativeSig P) (full_P : FullSig P) : forall {sts Γ M A B s1 s2 s3 s1' s2' } {r : Ru P s1 s2 s3},
-    {{ ⟪ pred_P ⟫ Γ : sts ⊩ A : Sort@s1 : s1' }} ->
-    {{ ⟪ pred_P ⟫ Γ, A : (s1 :: sts) ⊩ B : Sort@s2 : s2' }} ->
-    {{ ⟪ pred_P ⟫ Γ, A : (s1 :: sts) ⊩ M : B : s2 }} ->
-    {{ ⟪ pred_P ⟫ Γ : sts ⊩ λ r A M : Π r A B : s3 }}.
+Lemma glu_rel_exp_fn_helper {P} (pred_P : PredicativeSig P) (full_P : FullSig P) : forall {Γ M A B s1 s2 s3 s1' s2' } {r : Ru P s1 s2 s3},
+    {{ ⟪ pred_P ⟫ Γ ⊩ A : Sort@s1 > s1' }} ->
+    {{ ⟪ pred_P ⟫ Γ, A:Sort@s1 ⊩ B : Sort@s2 > s2' }} ->
+    {{ ⟪ pred_P ⟫ Γ, A:Sort@s1 ⊩ M : B > s2 }} ->
+    {{ ⟪ pred_P ⟫ Γ ⊩ λ r A M : Π r A B > s3 }}.
 Proof.
   intros * HA HB HM.
-  assert {{ ⟪ pred_P ⟫ ⊩ Γ : sts }} as [SbΓ] by mauto 3.
+  assert {{ ⟪ pred_P ⟫ ⊩ Γ }} as [SbΓ] by mauto 3.
   assert {{ Γ ⊢ A : Sort@s1 }} by mauto 3.
   inversion_clear HA as [SbΓ' []].  
   handle_functional_glu_ctx_env P.
   rename SbΓ' into SbΓ.
   pose (SbΓA := cons_glu_sub_pred pred_P s1 Γ A SbΓ).
-  assert {{ EG Γ, A ∈ glu_ctx_env pred_P (s1 :: sts) ↘ SbΓA }} by (econstructor; mauto 3; reflexivity).
-  assert {{ Γ, A ⊢ M : B }} by mauto 3.
+  assert {{ EG Γ, A:Sort@s1 ∈ glu_ctx_env pred_P ↘ SbΓA }} by (econstructor; mauto 3; reflexivity).
+  assert {{ Γ, A:Sort@s1 ⊢ M : B }} by mauto 3.
   inversion_clear HM as [SbΓA' []].
   handle_functional_glu_ctx_env P.
   rename SbΓA' into SbΓA.
-  assert {{ Γ, A ⊢ B : Sort@s2 }} by mauto.
-  assert {{ ⟪ pred_P ⟫ Γ, A ⊨u M : B }} as [env_relΓA] by mauto using completeness_fundamental_exp.
+  assert {{ Γ, A:Sort@s1 ⊢ B : Sort@s2 }} by mauto 3.
+  assert {{ ⟪ pred_P ⟫ Γ, A:Sort@s1 ⊨u M : B }} as [env_relΓA] by mauto using completeness_fundamental_exp.
   destruct_conjs.
   pose env_relΓA.
   match_by_head (per_ctx_env pred_P env_relΓA) invert_per_ctx_env.
@@ -207,6 +209,7 @@ Proof.
   assert {{ Δ ⊢s σ : Γ }} by mauto 4.
   assert {{ Dom ρ ≈ ρ ∈ env_relΓ }} by (eapply glu_ctx_env_per_env; revgoals; eassumption).
   destruct_rel_typ_unsorted.
+  destruct_rel_typ.
   destruct_glu_rel_exp_with_sub.
   simplify_evals.
   match_by_head (@glu_sort_elem P) ltac:(fun H => directed invert_glu_sort_elem H).
@@ -218,25 +221,26 @@ Proof.
   do 2 eexists; repeat split; mauto.
   intros.
   match_by_head (@glu_sort_elem P) ltac:(fun H => directed invert_glu_sort_elem H).
-  assert (glu_sort_elem pred_P s1 IP IEL a).
-  {
-    assert ((pred_rel pred_P s1 s3 \/ s1 = s3) /\ (pred_rel pred_P s2 s3 \/ s2 = s3)) as [pr1 pr2] by (eapply ord_ru; mauto 2).
-    destruct glu_a as [glu_a_eq glu_a_rel].
-    destruct pr1;
-      [eapply glu_a_rel | subst; eapply glu_a_eq]; mauto 2.    
-  }
-  assert (forall c (equiv_c : in_rel c c) b,
-             {{ ⟦ B ⟧ ρ ↦ c ↘ b }} ->
-             glu_sort_elem pred_P s2 (OP c equiv_c) (OEL c equiv_c) b).
-  {
-    assert ((pred_rel pred_P s1 s3 \/ s1 = s3) /\ (pred_rel pred_P s2 s3 \/ s2 = s3)) as [pr1 pr2] by (eapply ord_ru; mauto 2).
-    intros.
-    assert ((s2 = s3 -> glu_sort_elem pred_P s3 (OP c equiv_c) (OEL c equiv_c) b) /\
-              (pred_rel pred_P s2 s3 -> glu_sort_elem pred_P s2 (OP c equiv_c) (OEL c equiv_c) b)) as [glu_b_eq glu_b_rel] by mauto 2.
-    destruct pr2;
-      [eapply glu_b_rel | subst; eapply glu_b_eq]; mauto 2.
-  }
-  assert (per_typ_elem pred_P in_rel a a) by mauto 2.
+  rename H19 into IP, H20 into IEL, x into OP, x0 into OEL.
+  (* assert (glu_sort_elem pred_P s1 IP IEL a). *)
+  (* { *)
+  (*   assert ((pred_rel pred_P s1 s3 \/ s1 = s3) /\ (pred_rel pred_P s2 s3 \/ s2 = s3)) as [pr1 pr2] by (eapply ord_ru; mauto 2). *)
+  (*   destruct glu_a as [glu_a_eq glu_a_rel]. *)
+  (*   destruct pr1; *)
+  (*     [eapply glu_a_rel | subst; eapply glu_a_eq]; mauto 2.     *)
+  (* } *)
+  (* assert (forall c (equiv_c : in_rel c c) b, *)
+  (*            {{ ⟦ B ⟧ ρ ↦ c ↘ b }} -> *)
+  (*            glu_sort_elem pred_P s2 (OP c equiv_c) (OEL c equiv_c) b). *)
+  (* { *)
+  (*   assert ((pred_rel pred_P s1 s3 \/ s1 = s3) /\ (pred_rel pred_P s2 s3 \/ s2 = s3)) as [pr1 pr2] by (eapply ord_ru; mauto 2). *)
+  (*   intros. *)
+  (*   assert ((s2 = s3 -> glu_sort_elem pred_P s3 (OP c equiv_c) (OEL c equiv_c) b) /\ *)
+  (*             (pred_rel pred_P s2 s3 -> glu_sort_elem pred_P s2 (OP c equiv_c) (OEL c equiv_c) b)) as [glu_b_eq glu_b_rel] by mauto 2. *)
+  (*   destruct pr2; *)
+  (*     [eapply glu_b_rel | subst; eapply glu_b_eq]; mauto 2. *)
+  (* } *)
+  assert (per_typ_elem pred_P (head_rel ρ ρ H11) a a) by mauto 2.
   handle_per_typ_elem_irrel.
   handle_functional_glu_sort_elem P.
   match goal with
@@ -246,9 +250,9 @@ Proof.
   end.
   match_by_head (@per_sort_elem P) ltac:(fun H => directed invert_per_sort_elem H).
   apply_relation_equivalence.
-  assert {{ Δ, A[σ] ⊢ B[q σ] : Sort@s2 }} by mauto 3.
-  econstructor; mauto 3; intros.
-  - assert {{ Dom ρ ↦ n ≈ ρ ↦ n' ∈ env_relΓA }} as HrelΓA by (apply_relation_equivalence; mautosolve 2).
+  assert {{ Δ, A[σ]:Sort@s1 ⊢ B[q σ] : Sort@s2 }} by mauto 3.
+  econstructor; mauto 4; intros.
+  - assert {{ Dom ρ ↦ n ≈ ρ ↦ n' ∈ env_relΓA }} as HrelΓA by (apply_relation_equivalence; mautosolve 3).
     destruct_rel_mod_eval.
     apply_relation_equivalence.
     assert (exists elem_rel : relation (domain P),
@@ -274,22 +278,16 @@ Proof.
     assert {{ Δ0 ⊢ B[σ∘σ0,,N] ≈ B[q σ][σ0,,N] : Sort@s2 }} as <-.
     {
       gen_presups.
-      assert {{ Δ0 ⊢s q σ ∘ (σ0 ,, N) ≈ σ ∘ σ0 ,, N : Γ, A }} by (eapply sub_decompose_q; mauto 2).
-      transitivity {{{ B[(q σ)∘(σ0,,N)] }}}.
-      - eapply eq_exp_eq_sub_typ; mauto 3.
-        econstructor; mauto 3.
-        econstructor; mauto 3.
-        econstructor; mauto 3.
-      - eapply exp_eq_sub_compose_typ_sort; mauto 3.
-        + eapply sub_q; mauto 2.
-        + econstructor; mauto 2.
+      assert {{ Δ0 ⊢s q σ ∘ (σ0 ,, N) ≈ σ ∘ σ0 ,, N : Γ, A:Sort@s1 }} by (eapply sub_decompose_q; mauto 2).
+      transitivity {{{ B[(q σ)∘(σ0,,N)] }}}; mauto 3.
+      eapply wf_exp_eq_sub_compose_sort; mauto 3.
     }    
 
     assert {{ Δ0 ⊢ (λ r A M)[σ][σ0] N ≈ M[(σ∘σ0),,N] : B[σ∘σ0,,N] }} as ->.
     {
       assert {{ Δ0 ⊢s σ∘σ0 : Γ }} by mauto 3.
-      assert {{ Δ0, A[σ∘σ0] ⊢ M[q (σ∘σ0)] : B[q (σ∘σ0)] }} by mauto 3.
-      assert {{ Δ0 ⊢ (λ r A M)[σ][σ0] ≈ (λ r A M)[σ∘σ0] : (Π r A B)[σ∘σ0] }} by (symmetry; mauto 3).
+      assert {{ Δ0, A[σ∘σ0]:Sort@s1 ⊢ M[q (σ∘σ0)] : B[q (σ∘σ0)] }} by mauto 3.
+      assert {{ Δ0 ⊢ (λ r A M)[σ][σ0] ≈ (λ r A M)[σ∘σ0] : (Π r A B)[σ∘σ0] }} by (symmetry; mauto 4).
       assert {{ Δ0 ⊢ (λ r A M)[σ][σ0] ≈ (λ r A[σ∘σ0] M[q (σ∘σ0)]) : (Π r A B)[σ∘σ0] }} by mauto 3.
       assert {{ Δ0 ⊢ (λ r A M)[σ][σ0] ≈ (λ r A[σ∘σ0] M[q (σ∘σ0)]) : Π r A[σ∘σ0] B[q (σ∘σ0)] }} by mauto 4.
       assert {{ Δ0 ⊢ N : A[σ∘σ0] }} by mauto 4.
@@ -300,9 +298,9 @@ Proof.
         eapply wf_exp_eq_pi_beta'; mauto 3.
       }
       transitivity {{{ M[q (σ∘σ0)][Id,,N] }}}; [mauto 4 |].
-      assert {{ Δ0 ⊢s Id,,N : Δ0, A[σ∘σ0] }} by mauto 3.
-      assert {{ Δ0, A[σ∘σ0] ⊢s q (σ∘σ0) : Γ, A }} by mauto 2.
-      assert {{ Δ0 ⊢s q (σ∘σ0)∘(Id,,N) ≈ σ∘σ0,,N : Γ, A }} by mauto 2.
+      assert {{ Δ0 ⊢s Id,,N : Δ0, A[σ∘σ0]:Sort@s1 }} by mauto 3.
+      assert {{ Δ0, A[σ∘σ0]:Sort@s1 ⊢s q (σ∘σ0) : Γ, A:Sort@s1 }} by mauto 2.
+      assert {{ Δ0 ⊢s q (σ∘σ0)∘(Id,,N) ≈ σ∘σ0,,N : Γ, A:Sort@s1 }} by mauto 2.
       assert {{ Δ0 ⊢ B[q (σ∘σ0)∘(Id,,N)] ≈ B[σ∘σ0,,N] : Sort@s2 }} as <- by mauto 4.
       transitivity {{{ M[q (σ∘σ0)∘(Id,,N)] }}}; mauto 3.
     }
@@ -310,7 +308,7 @@ Proof.
     assert {{ Δ0 ⊢s (σ∘σ0),,N ® ρ ↦ n ∈ SbΓA }} as HSbΓA.
     {
       assert (SbΓA <∙> cons_glu_sub_pred pred_P s1 Γ A SbΓ) by (eapply glu_ctx_env_cons_clean_inversion; mauto 3).
-      eapply H40.
+      eapply H36.
       mauto 3.
     }
     (on_all_hyp: fun H => destruct (H _ _ _ HSbΓA)).
@@ -320,31 +318,31 @@ Proof.
     mauto 3.
 Qed.
 
-Lemma glu_rel_exp_fn {P} (pred_P : PredicativeSig P) (full_P : FullSig P) : forall {sts Γ M A B s1 s2 s3 s1'} {r : Ru P s1 s2 s3},
-    {{ ⟪ pred_P ⟫ Γ : sts ⊩ A : Sort@s1 : s1' }} ->
-    {{ ⟪ pred_P ⟫ Γ, A : (s1 :: sts) ⊩ M : B : s2 }} ->
-    {{ ⟪ pred_P ⟫ Γ : sts ⊩ λ r A M : Π r A B : s3 }}.
+Lemma glu_rel_exp_fn {P} (pred_P : PredicativeSig P) (full_P : FullSig P) : forall {Γ M A B s1 s2 s3 s1'} {r : Ru P s1 s2 s3},
+    {{ ⟪ pred_P ⟫ Γ ⊩ A : Sort@s1 > s1' }} ->
+    {{ ⟪ pred_P ⟫ Γ, A:Sort@s1 ⊩ M : B > s2 }} ->
+    {{ ⟪ pred_P ⟫ Γ ⊩ λ r A M : Π r A B > s3 }}.
 Proof.
   intros * HA HM.
-  assert (exists s2', {{ ⟪ pred_P ⟫ Γ, A : (s1 :: sts) ⊩ B : Sort@s2 : s2' }}) as [s2'] by mauto 3.
-  assert {{ ⟪ pred_P ⟫ ⊩ Γ : sts }} by mauto 3.
-  assert {{ ⟪ pred_P ⟫ ⊩ Γ, A : (s1 :: sts) }} by mauto 3.
+  assert (exists s2', {{ ⟪ pred_P ⟫ Γ, A:Sort@s1 ⊩ B : Sort@s2 > s2' }}) as [s2'] by mauto 3.
+  assert {{ ⟪ pred_P ⟫ ⊩ Γ }} by mauto 3.
+  assert {{ ⟪ pred_P ⟫ ⊩ Γ, A:Sort@s1 }} by mauto 3.
   mauto 3 using glu_rel_exp_fn_helper.
 Qed.
 
 #[export]
 Hint Resolve glu_rel_exp_fn : mcpts.
 
-Lemma glu_rel_exp_app_helper {P} (pred_P : PredicativeSig P) (full_P : FullSig P) : forall {sts Γ M N A B s1 s2 s3 s1' s2'} {r : Ru P s1 s2 s3},
-    {{ ⟪ pred_P ⟫ Γ : sts ⊩ A : Sort@s1 : s1' }} ->
-    {{ ⟪ pred_P ⟫ Γ, A : (s1 :: sts) ⊩ B : Sort@s2 : s2' }} ->
-    {{ ⟪ pred_P ⟫ Γ : sts ⊩ M : Π r A B : s3 }} ->
-    {{ ⟪ pred_P ⟫ Γ : sts ⊩ N : A : s1 }} ->
-    {{ ⟪ pred_P ⟫ Γ : sts ⊩ M N : B[Id,,N] : s2 }}.
+Lemma glu_rel_exp_app_helper {P} (pred_P : PredicativeSig P) (full_P : FullSig P) : forall {Γ M N A B s1 s2 s3 s1' s2'} {r : Ru P s1 s2 s3},
+    {{ ⟪ pred_P ⟫ Γ ⊩ A : Sort@s1 > s1' }} ->
+    {{ ⟪ pred_P ⟫ Γ, A:Sort@s1 ⊩ B : Sort@s2 > s2' }} ->
+    {{ ⟪ pred_P ⟫ Γ ⊩ M : Π r A B > s3 }} ->
+    {{ ⟪ pred_P ⟫ Γ ⊩ N : A > s1 }} ->
+    {{ ⟪ pred_P ⟫ Γ ⊩ M N : B[Id,,N] > s2 }}.
 Proof.
   intros * HA HB HM HN.
-  assert {{ ⟪ pred_P ⟫ ⊩ Γ : sts }} as [SbΓ] by mauto 3.
-  assert (exists s3', {{ ⟪ pred_P ⟫ Γ : sts ⊩ Π r A B : Sort@s3 : s3' }}) as [s3'] by mauto 4.
+  assert {{ ⟪ pred_P ⟫ ⊩ Γ }} as [SbΓ] by mauto 3.
+  assert (exists s3', {{ ⟪ pred_P ⟫ Γ ⊩ Π r A B : Sort@s3 > s3' }}) as [s3'] by mauto 4.
   assert {{ Γ ⊢ N : A }} by mauto 2.
   inversion_clear HN as [SbΓ' []].
   handle_functional_glu_ctx_env P.
@@ -353,7 +351,7 @@ Proof.
   inversion_clear HA as [SbΓ' []].
   handle_functional_glu_ctx_env P.
   pose (SbΓA := cons_glu_sub_pred pred_P s1 Γ A SbΓ).
-  assert {{ EG Γ, A ∈ glu_ctx_env pred_P (s1 :: sts) ↘ SbΓA }}.
+  assert {{ EG Γ, A:Sort@s1 ∈ glu_ctx_env pred_P ↘ SbΓA }}.
   {
     econstructor; mauto 3; try reflexivity.
     intros.
@@ -362,7 +360,7 @@ Proof.
     eapply H7.
     eassumption.
   }
-  assert {{ Γ, A ⊢ B : Sort@s2 }} by mauto 2.
+  assert {{ Γ, A:Sort@s1 ⊢ B : Sort@s2 }} by mauto 2.
   inversion_clear HB as [SbΓA' []].
   handle_functional_glu_ctx_env P.
   rename SbΓA' into SbΓA.
@@ -467,8 +465,8 @@ Proof.
   assert {{ Δ ⊢s σ : Γ }} by mauto 2.
   assert {{ Δ ⊢ N[σ] : A[σ] }} by mauto 2.
   assert {{ Δ ⊢ B[Id,,N][σ] ≈ B[(Id,,N)∘σ] : Sort@s2 }} by (symmetry; mauto 4).
-  assert {{ Δ ⊢s (Id,,N)∘σ ≈ σ,,N[σ] : Γ, A }} by mauto 3.
-  assert {{ Δ ⊢ B[(Id,,N)∘σ] ≈ B[σ,,N[σ]] : Sort@s2 }} by (eapply eq_exp_eq_sub_typ; mauto 3).
+  assert {{ Δ ⊢s (Id,,N)∘σ ≈ σ,,N[σ] : Γ, A:Sort@s1 }} by mauto 3.
+  assert {{ Δ ⊢ B[(Id,,N)∘σ] ≈ B[σ,,N[σ]] : Sort@s2 }} by mauto 3. 
   assert {{ Δ ⊢ B[Id,,N][σ] ≈ B[σ,,N[σ]] : Sort@s2 }} as -> by mauto 3.
   assert {{ Δ ⊢ (M N)[σ] ≈ M[σ] N[σ] : B[σ,,N[σ]] }} as -> by mauto 2.
   assert {{ Δ ⊢ M[σ][Id] N[σ] ≈ M[σ] N[σ] : B[σ,,N[σ]] }} as <-.
@@ -485,29 +483,30 @@ Proof.
   eapply glu_sort_elem_typ_unique_upto_exp_eq; revgoals; eassumption.
 Qed.
 
-Lemma glu_rel_exp_app {P} (pred_P : PredicativeSig P) (full_P : FullSig P) : forall {sts Γ M N A B s1 s2 s3 s2'} {r : Ru P s1 s2 s3},
-    {{ ⟪ pred_P ⟫ Γ, A : (s1 :: sts) ⊩ B : Sort@s2 : s2' }} ->
-    {{ ⟪ pred_P ⟫ Γ : sts ⊩ M : Π r A B : s3 }} ->
-    {{ ⟪ pred_P ⟫ Γ : sts ⊩ N : A : s1 }} ->
-    {{ ⟪ pred_P ⟫ Γ : sts ⊩ M N : B[Id,,N] : s2 }}.
+Lemma glu_rel_exp_app {P} (pred_P : PredicativeSig P) (full_P : FullSig P) : forall {Γ M N A B s1 s2 s3 s2'} {r : Ru P s1 s2 s3},
+    {{ ⟪ pred_P ⟫ Γ, A:Sort@s1 ⊩ B : Sort@s2 > s2' }} ->
+    {{ ⟪ pred_P ⟫ Γ ⊩ M : Π r A B > s3 }} ->
+    {{ ⟪ pred_P ⟫ Γ ⊩ N : A > s1 }} ->
+    {{ ⟪ pred_P ⟫ Γ ⊩ M N : B[Id,,N] > s2 }}.
 Proof.
   intros * HB HM HN.
-  assert {{ ⟪ pred_P ⟫ ⊩ Γ, A : (s1 :: sts) }} as [SbΓA] by mauto 3.
-  match_by_head (glu_ctx_env pred_P (s1 :: sts) SbΓA) invert_glu_ctx_env.
+  assert {{ ⟪ pred_P ⟫ ⊩ Γ, A:Sort@s1 }} as [SbΓA] by mauto 3.
+  match_by_head (glu_ctx_env pred_P SbΓA) invert_glu_ctx_env.
   apply_predicate_equivalence.
   rename TSb into SbΓ.
   assert (exists s1', Ax P s1 s1') as [s1'] by (eapply full_P).
-  assert {{ ⟪ pred_P ⟫ Γ : sts ⊩ A : Sort@s1 : s1' }}.
+  assert {{ ⟪ pred_P ⟫ Γ ⊩ A : Sort@s1 > s1' }}.
   {
     eexists.
     intuition.
     destruct_glu_rel_typ_with_sub.
     econstructor; mauto 4.
     econstructor; [| split]; mauto 3.
+    eapply wf_exp_sub_typ; mauto 3.
     do 2 eexists; mauto 2.
   }
-  assert {{ ⟪ pred_P ⟫ ⊩ Γ : sts }} by mauto 2.
-  assert {{ ⟪ pred_P ⟫ ⊩ Γ, A : (s1 :: sts) }} by mauto 3.
+  assert {{ ⟪ pred_P ⟫ ⊩ Γ }} by mauto 2.
+  assert {{ ⟪ pred_P ⟫ ⊩ Γ, A:Sort@s1 }} by mauto 3.
   mauto 2 using glu_rel_exp_app_helper.
 Qed.
 
