mechanization/theories/Core/Soundness/FundamentalTheorem.v
@@ -12,64 +12,69 @@ Import Domain_Notations.
 
 Section soundness_fundamental.
   #[local]
-  Ltac gen_soundness_IH P pred_P full_P soundness_ctx soundness_exp soundness_sub H :=
+  Ltac gen_soundness_IH P pred_P full_P soundness_ctx soundness_exp soundness_typ soundness_sub H :=
   match type of H with
-  | {{ ⊫ ^?Γ > ?sts }} =>
+  | {{ ⊢ ^?Γ }} =>
       let HΓ := fresh "HΓ" in
-      pose proof soundness_ctx P pred_P full_P Γ sts H as HΓ
-  | {{ ^?Γ : ?sts ⊫ ^?M : ^?A > ?s }} =>
+      pose proof soundness_ctx P pred_P full_P Γ H as HΓ
+  | {{ ^?Γ ⊫ ^?M : ^?A > ^?s }} =>
       let HM := fresh "HM" in
-      pose proof soundness_exp P pred_P full_P Γ sts A s M H as HM
-  | {{ ^?Γ : ?stsΓ ⊫s ^?σ : ^?Δ > ?stsΔ }} =>
+      pose proof soundness_exp P pred_P full_P Γ A s M H as HM
+  | {{ ^?Γ ⊫ ^?A > ^?s }} =>
+      let HA := fresh "HA" in
+      pose proof soundness_typ P pred_P full_P Γ A s H as HA
+  | {{ ^?Γ ⊢s ^?σ : ^?Δ }} =>
       let Hσ := fresh "Hσ" in
-      pose proof soundness_sub P pred_P full_P Γ stsΓ Δ stsΔ σ H as Hσ
+      pose proof soundness_sub P pred_P full_P Γ Δ σ H as Hσ
   end.
    
   Theorem soundness_fundamental_ctx_ann {P} (pred_P : PredicativeSig P) (full_P : FullSig P) :
-    forall Γ sts, {{ ⊫ Γ > sts }} -> {{ ⟪ pred_P ⟫ ⊩ Γ : sts }}
+    forall Γ, {{ ⊢ Γ }} -> {{ ⟪ pred_P ⟫ ⊩ Γ }}
   with soundness_fundamental_exp_ann {P} (pred_P : PredicativeSig P) (full_P : FullSig P) :
-    forall Γ sts A s M, {{ Γ : sts ⊫ M : A > s }} -> {{ ⟪ pred_P ⟫ Γ : sts ⊩ M : A : s }}
+    forall Γ A s M, {{ Γ ⊫ M : A > s }} -> {{ ⟪ pred_P ⟫ Γ ⊩ M : A > s }}
+  with soundness_fundamental_typ_ann {P} (pred_P : PredicativeSig P) (full_P : FullSig P) :
+    forall Γ A s, {{ Γ ⊫ A > s }} -> {{ ⟪ pred_P ⟫ Γ ⊩ A > s }}
   with soundness_fundamental_sub_ann {P} (pred_P : PredicativeSig P) (full_P : FullSig P) :
-    forall Γ stsΓ Δ stsΔ σ, {{ Γ : stsΓ ⊫s σ : Δ > stsΔ }} -> {{ ⟪ pred_P ⟫ Γ : stsΓ ⊩s σ : Δ : stsΔ }}.
+    forall Γ Δ σ, {{ Γ ⊢s σ : Δ }} -> {{ ⟪ pred_P ⟫ Γ ⊩s σ : Δ }}.
   Proof.
     all: inversion_clear 1;
-      (on_all_hyp: gen_soundness_IH P pred_P full_P soundness_fundamental_ctx_ann soundness_fundamental_exp_ann soundness_fundamental_sub_ann);
-      clear soundness_fundamental_ctx_ann soundness_fundamental_exp_ann soundness_fundamental_sub_ann;
+      (on_all_hyp: gen_soundness_IH P pred_P full_P soundness_fundamental_ctx_ann soundness_fundamental_exp_ann soundness_fundamental_typ_ann soundness_fundamental_sub_ann);
+      clear soundness_fundamental_ctx_ann soundness_fundamental_exp_ann soundness_fundamental_typ_ann soundness_fundamental_sub_ann;
       mauto 2.
 
-    - (* assert (exists Γ' A', (Γ = {{{ Γ', A' }}})) as [Γ' [A' ->]]. *)
-      (* { *)
-      (*   destruct H1; do 2 eexists; mauto 2. *)
-      (* } *)
-      (* destruct HM as [SbΓ' []]. *)
-      (* eexists; split; eauto. *)
-      (* invert_glu_ctx_env H.       *)
-      (* intros. *)
-      (* destruct_glu_rel_exp_with_sub.       *)
-      (* simplify_evals. *)
-      (* rewrite H2 in H7. *)
-      (* inversion_clear H7. *)
-      (* inversion H14. *)
-      (* subst. *)
-      (* rename a into a'. *)
-      (* rename m into a. *)
-      (* econstructor; mauto 3. *)
-      (* + econstructor; mauto 3. *)
-        
+    - (* Context extensions. Need to define proper annotations {{ ⊫ Γ }} *)
       admit.
-
-    (* Cases for naturals ignored since they will be removed in FSCD *)
-    - admit.
-    - admit.
-    - admit.
-    - admit.
-
-    (* Cases for conversion rules, hard *)
-    - enough {{ Γ ⊢ A0 ≈ A : Sort@s }} by (eapply glu_rel_exp_conv'; mauto 2).
+    - (* wf_typ_sort *)
+      assert (exists s', Ax P s s') as [s'] by (eapply full_P).
+      assert {{ ⟪ pred_P ⟫ Γ ⊩ Sort@s0 : Sort@s > s' }} by mauto 2.
+      destruct H2 as [SbΓ []].
+      econstructor; split; mauto 2.
+      intros.
+      destruct_glu_rel_exp_with_sub.
+      simplify_evals.
+      invert_glu_sort_elem H7.
+      unfold sort_glu_exp_pred' in *.
+      unfold glu_sort_typ_rec in *.
+      eapply H6 in H8.
+      destruct_conjs.      
+      econstructor; mauto 2.      
+      
+    - (* wf_typ_exp *)
+      destruct HM as [SbΓ []].
+      eexists; split; mauto 2.
+      intros.
+      destruct_glu_rel_exp_with_sub.
+      simplify_evals.
+      invert_glu_sort_elem H5.
+      unfold sort_glu_exp_pred' in *.
+      unfold glu_sort_typ_rec in *.
+      eapply H5 in H6.
+      destruct_conjs.      
+      econstructor; mauto 2.
+    - (* Substitution extensions (need to properly define annotated judgments {{ Γ ⊫s σ : Δ }} *)
       admit.
-    - admit.
-    - admit.
-    - admit.
+    - (* Conversion for substitutions (need another lemma) *)
+      admit.
       
   Admitted.
   
