mechanization/theories/Core/Soundness/Realizability.v
@@ -8,27 +8,27 @@ Import Domain_Notations.
 
 Open Scope list_scope.
 
-Lemma wf_ctx_sub_ctx_lookup {P} : forall n (A : typ P) Γ,
-    {{ #n : A ∈ Γ }} ->
+Lemma wf_ctx_sub_ctx_lookup {P} : forall n (A : typ P) s Γ,
+    {{ #n : A : Sort@s ∈ Γ }} ->
     forall Δ,
       {{ ⊢ Δ ≈ Γ }} ->
       exists Δ1 A0 Δ2 A',
-        Δ = Δ1 ++ A0 :: Δ2 /\
+        Δ = Δ1 ++ (A0, {{{ Sort@s }}}) :: Δ2 /\
           n = length Δ1 /\
           A' = iter (S n) (fun A => {{{ A[Wk] }}}) A0 /\
-          {{ #n : A' ∈ Δ }} /\
-          {{ Δ ⊢ A' ≈ A }}.
+          {{ #n : A' : Sort@s ∈ Δ }} /\
+          {{ Δ ⊢ A' ≈ A : Sort@s }}.
 Proof.
   induction 1; intros; progressive_inversion.
   - exists nil.
     repeat eexists; mauto 4.
   - edestruct IHctx_lookup as [Δ1 [? [? [? [? [? [? []]]]]]]]; mauto.
-    exists (A0 :: Δ1). subst.
+    exists ((A0, {{{ Sort@s1 }}}) :: Δ1). subst.
     repeat eexists; mauto 4.
 Qed.
 
-Lemma var_arith {P} : forall (Γ1 Γ2 : ctx P) (A : typ P),
-    length (Γ1 ++ A :: Γ2) - length Γ2 - 1 = length Γ1.
+Lemma var_arith {P} : forall (Γ1 Γ2 : ctx P) (A : typ P) s,
+    length (Γ1 ++ (A, {{{ Sort@s }}}) :: Γ2) - length Γ2 - 1 = length Γ1.
 Proof.
   intros.
   rewrite List.app_length. simpl.
@@ -37,72 +37,74 @@ Qed.
 
 Lemma var_weaken_gen {P} : forall (Δ : ctx P) (σ : sub P) (Γ : ctx P),
     {{ Δ ⊢w σ : Γ }} ->
-    forall Γ1 Γ2 A0,
-      Γ = Γ1 ++ A0 :: Γ2 ->
+    forall Γ1 Γ2 A0 s0,
+      Γ = Γ1 ++ (A0, {{{ Sort@s0 }}}) :: Γ2 ->
       {{ Δ ⊢ #(length Γ1)[σ] ≈ #(length Δ - length Γ2 - 1) : ^(iter (S (length Γ1)) (fun A => {{{ A[Wk] }}}) A0)[σ] }}.
-Proof.  
+Proof.
   induction 1; intros; subst; gen_presups.
-  - pose proof (app_ctx_vlookup _ _ _ _ ltac:(eassumption) eq_refl) as Hvar.
-
+  - pose proof (app_ctx_vlookup _ _ _ _ _ ltac:(eassumption) eq_refl) as Hvar.
+    
     (* gen_presup Hvar. *)
-    assert {{ ⊢ ^ (app Γ1 {{{ Γ2, A0 }}}) }} by mauto.
-    assert {{ ^(app Γ1 {{{ Γ2, A0 }}}) ⊢ ^(iter (S (length Γ1)) (fun T : exp P => {{{ T[Wk] }}}) A0) }} by (eapply presup_exp_typ; mauto).   
+    pose proof (app_ctx_lookup Γ1 A0 Γ2 (length Γ1) s0 ltac:(reflexivity)).
+    assert {{ ⊢ ^ (app Γ1 {{{ Γ2, A0:Sort@s0 }}}) }} by mauto.
+    pose proof (presup_ctx_lookup_typ H1 H0).
+    assert {{ ^(app Γ1 {{{ Γ2, A0:Sort@s0 }}}) ⊢ ^(iter (S (length Γ1)) (fun T : exp P => {{{ T[Wk] }}}) A0) }} by (eapply presup_exp_typ; mauto).   
     clear_dups.
     apply wf_sub_id_inversion in Hτ.
     pose proof (wf_ctx_sub_length _ _ Hτ).
-    transitivity {{{ #(length Γ1)[^(@a_id P)] }}}; [mauto 3 |].
-    replace (length Γ) with (length (Γ1 ++ {{{ Γ2, A0 }}})) by lia.
+    transitivity {{{ #(length Γ1)[^(@a_id P)] }}}; mauto 3.
+    replace (length Γ) with (length (Γ1 ++ {{{ Γ2, A0:Sort@s0 }}})) by lia.
     rewrite var_arith.
-    eapply wf_exp_eq_conv; [eapply wf_exp_eq_sub_id; mauto | mauto |].
+    eapply wf_exp_eq_conv'; [eapply wf_exp_eq_sub_id; mauto 3 |].
     transitivity {{{ ^(iter (S (length Γ1)) (fun T : exp P => {{{ T[Wk] }}}) A0)[Id] }}}; mauto.
 
-  - pose proof (app_ctx_vlookup _ _ _ _ HΔ0 eq_refl) as Hvar.
-    pose proof (app_ctx_lookup Γ1 A0 Γ2 _ eq_refl).
+  - pose proof (app_ctx_vlookup _ _ _ _ _ HΔ0 eq_refl) as Hvar.
+    pose proof (app_ctx_lookup Γ1 A0 Γ2 _ s0 eq_refl).
 
-    gen_presup Hvar.
+    (* gen_presup Hvar. *)
     clear_dups.
-    assert {{ ⊢ Δ', A }} by mauto 3.
-    assert {{ Δ', A ⊢s Wk : ^(Γ1 ++ {{{ Γ2, A0 }}}) }} by mauto 3.
-    transitivity {{{ #(length Γ1)[Wk∘τ] }}}; [mauto 3 |].
-    eapply wf_exp_eq_conv' with (A := {{{ ^ (iter (S (length Γ1)) (fun A1 : exp P => {{{ A1[Wk] }}}) A0)[Wk∘τ] }}}); mauto 3.
+    assert {{ ⊢ Δ', A:Sort@s }} by mauto 3.
+    assert {{ Δ', A:Sort@s ⊢s Wk : ^(Γ1 ++ {{{ Γ2, A0:Sort@s0 }}}) }} by mauto 3.
+    transitivity {{{ #(length Γ1)[Wk∘τ] }}}; [mauto 4 |].
+    eapply wf_exp_eq_conv' with (A := {{{ ^ (iter (S (length Γ1)) (fun A1 : exp P => {{{ A1[Wk] }}}) A0)[Wk∘τ] }}}); mauto 4.
     
-    etransitivity; [eapply wf_exp_eq_sub_compose; mauto 3 |].
+    etransitivity; [eapply wf_exp_eq_sub_compose_typ; mauto 3 |].
     pose proof (wf_ctx_sub_length _ _ H0).
 
-    eapply wf_exp_eq_conv' with {{{ ^ (iter (S (length Γ1)) (fun A1 : exp P => {{{ A1[Wk] }}}) A0)[Wk][τ] }}}; mauto 3.
+    eapply wf_exp_eq_conv' with (A := {{{ ^ (iter (S (length Γ1)) (fun A1 : exp P => {{{ A1[Wk] }}}) A0)[Wk][τ] }}}); mauto 4.
 
     deepexec (@wf_ctx_sub_ctx_lookup P) ltac:(fun H => destruct H as [Γ1' [? [Γ2' [? [-> [? [-> []]]]]]]]).
     repeat rewrite List.app_length in *.
-    replace (length Γ1) with (length Γ1') in * by lia.
-    clear_refl_eqs.
-    replace (length Γ2) with (length Γ2') by (simpl in *; lia).
 
     etransitivity.
-    + eapply wf_exp_eq_sub_cong; [ |mauto 3].
-      eapply wf_exp_eq_conv'.
+    + assert {{ ⊢ ^ (app Γ1' {{{ Γ2',x:Sort@s0 }}}) }} by mauto 3.
+      eapply wf_exp_eq_sub_cong_typ; [| eapply wf_exp_eq_conv' |mauto 3].      
+      * eapply wf_exp_sub_sort; mauto 2.
       * eapply wf_exp_eq_var_weaken; [mauto 3|]; eauto.
       * mauto 4.
-    + eapply wf_exp_eq_conv'.
-      * eapply IHweakening with (Γ1 := A :: _).
+    + replace (length Γ1) with (length Γ1') in * by lia.
+      clear_refl_eqs.
+      replace (length Γ2) with (length Γ2') by (simpl in *; lia).
+      eapply wf_exp_eq_conv'.
+      * eapply IHweakening with (Γ1 := (A, {{{ Sort@s }}}) :: _).
         reflexivity.
-      * eapply wf_subtyp_subst; [ |mauto 3].
-        simpl. eapply wf_subtyp_subst; mauto 3.
+      * eapply wf_exp_eq_sub_cong_sort; mauto 3.
 Qed.
 
 Lemma var_glu_elem_bot {P} (pred_P : PredicativeSig P) : forall a s typ_rel exp_rel Γ A,
     {{ DG a ∈ glu_sort_elem pred_P s ↘ typ_rel ↘ exp_rel }} ->
     typ_rel Γ A ->
     (* {{ Γ ⊢ A ® P }} -> *)
-    glu_elem_bot pred_P s a {{{ Γ, A }}} {{{ A[Wk] }}} {{{ #0 }}} (d_var (length Γ) ).
+    glu_elem_bot pred_P s a {{{ Γ, A:Sort@s }}} {{{ A[Wk] }}} {{{ #0 }}} (d_var (length Γ) ).
     (* {{ Γ, A ⊢ #0 : A[Wk] ® !(length Γ) ∈ glu_elem_bot pred_P s a }}. *)
 Proof.
   intros. saturate_glu_info.
   econstructor; mauto 4.
   - eapply glu_sort_elem_typ_monotone; eauto.
-    assert {{ ⊢ Γ, A }} by mauto 3.
+    assert {{ ⊢ Γ, A:Sort@s }} by mauto 3.
     eapply weakening_wk; mauto 3.
   - intros. progressive_inversion.
-    exact (var_weaken_gen _ _ _ H2 nil _ _ eq_refl).
+    exact (var_weaken_gen _ _ _ H2 nil _ _ _ eq_refl).
 Qed.
 
 #[local]
@@ -187,14 +189,14 @@ Proof.
       destruct_rel_mod_eval.
       simplify_evals.
       destruct (H2 _ ltac:(eassumption) _ ltac:(eassumption)) as [? []].
-      assert (IEL {{{ Δ, IT[σ] }}} {{{ IT[σ][Wk] }}} {{{ #0 }}} d{{{ ⇑! a (length Δ) }}}) by mauto 3 using var_glu_elem_bot.
-      assert {{ Δ, IT[σ] ⊢ IT[σ][Wk] ≈ IT[σ∘Wk] : Sort@s1 }}.
+      assert (IEL {{{ Δ, IT[σ]:Sort@s1 }}} {{{ IT[σ][Wk] }}} {{{ #0 }}} d{{{ ⇑! a (length Δ) }}}) by mauto 3 using var_glu_elem_bot.
+      assert {{ Δ, IT[σ]:Sort@s1 ⊢ IT[σ][Wk] ≈ IT[σ∘Wk] : Sort@s1 }}.
       {
         symmetry.
         eapply exp_eq_sub_compose_typ_sort; mauto.
       }
-      assert (IEL {{{ Δ,IT[σ] }}} {{{ IT[σ∘Wk] }}} {{{ #0 }}} d{{{ ⇑! a (length Δ) }}}) by (eapply glu_sort_elem_trm_resp_typ_exp_eq; mauto 2).
-      specialize (H14 {{{ Δ, IT[σ] }}} {{{ σ∘Wk }}} _ _ ltac:(mauto) ltac:(eassumption) ltac:(eassumption)).
+      assert (IEL {{{ Δ,IT[σ]:Sort@s1 }}} {{{ IT[σ∘Wk] }}} {{{ #0 }}} d{{{ ⇑! a (length Δ) }}}) by (eapply glu_sort_elem_trm_resp_typ_exp_eq; mauto 2).
+      specialize (H14 {{{ Δ, IT[σ]:Sort@s1 }}} {{{ σ∘Wk }}} _ _ ltac:(mauto) ltac:(eassumption) ltac:(eassumption)).
       specialize (H8 _ _ _ ltac:(eassumption) ltac:(eassumption)) as [].
       etransitivity; [| eapply H33]; mauto 3.
   - handle_functional_glu_sort_elem P.
@@ -210,6 +212,7 @@ Proof.
     simplify_evals.
     eexists; repeat split; mauto 3.
     eapply H2; eauto.
+    assert (HAs3: {{ Γ ⊢ A : Sort@s3 }}) by (gen_presup H4; mauto 2).
     assert {{ Δ ⊢ M[σ] : A[σ] }} by mauto 3.
     bulky_rewrite_in H23.
     unshelve (econstructor; eauto).
@@ -228,37 +231,44 @@ Proof.
       {
         (* assert {{ Δ0 ⊢ OT[(σ,,N)∘σ0] ≈ OT[σ,,N][σ0] : Sort@s2 }} by mauto 4. *)
         transitivity {{{ OT[(σ,,N)∘σ0] }}}; mauto 4.
-        assert {{ Δ0 ⊢s σ∘σ0,,N[σ0] ≈ (σ,,N)∘σ0 : Γ, IT }} by (econstructor; mauto 2).
-        gen_presup H.
-        eapply wf_exp_eq_conv' with (A:= {{{ Sort@s2[σ∘σ0,,N[σ0]] }}}); econstructor; mauto 2.
+        (* assert {{ Δ0 ⊢s σ∘σ0,,N[σ0] ≈ (σ,,N)∘σ0 : Γ, IT:Sort@s1 }} by mauto 4. (econstructor; mauto 2). *)
+        (* gen_presup H. *)
+        (* eapply wf_exp_eq_conv' with (A:= {{{ Sort@s2[σ∘σ0,,N[σ0]] }}}); econstructor; mauto 2. *)
       }
       enough {{ Δ0 ⊢ (M[σ] N)[σ0] ≈ ^ n{{{ M0 N0 }}} : OT[σ∘σ0,,N[σ0]] }} by mauto.
 
       etransitivity.
-      * assert (wf_typ_eq Δ0 {{{ OT[σ∘σ0,,N[σ0]] }}} {{{ OT[q σ][σ0,,N[σ0]] }}}) by (eapply sub_decompose_q_typ; mauto 3).
+      * assert {{ Δ0 ⊢ OT[σ∘σ0,,N[σ0]] ≈ OT[q σ][σ0,,N[σ0]] : Sort@s2 }} by (eapply sub_decompose_q_typ; mauto 3).
         eapply wf_exp_eq_conv' with (A:= {{{ OT[q σ][σ0,,N[σ0]] }}}); mauto 3.
       * simpl.
         rewrite <- @sub_eq_q_sigma_id_extend; mauto 4.
-        assert (wf_typ_eq Δ0 {{{ OT[q (σ∘σ0)][(Id,,N[σ0])] }}} {{{ OT[q (σ∘σ0)∘(Id,,N[σ0])] }}}).
+        assert {{ Δ0 ⊢ OT[q (σ∘σ0)][(Id,,N[σ0])] ≈ OT[q (σ∘σ0)∘(Id,,N[σ0])] : Sort@s2 }}.
         {
-          eapply exp_eq_sub_compose_typ; mauto 4.
-          assert (wf_sub Δ0 Δ0 (@a_id P)) by mauto 3.
-          assert (wf_exp Δ0 {{{ IT[σ][σ0] }}} {{{ N[σ0] }}}) by mauto 3.
-          assert (wf_typ_eq Δ0 {{{ IT[σ][σ0] }}} {{{ IT[σ∘σ0] }}}) by mauto 3.
-          gen_presup H35.
-          econstructor; mauto 3.
+          symmetry.
+          assert {{ Δ0 ⊢ IT[σ][σ0][Id] ≈ IT[σ][σ0] : Sort@s1 }} by mauto 4.
+          assert {{ Δ0 ⊢ N[σ0] : IT[σ][σ0] }} by mauto 3.
+          assert {{ Δ0 ⊢ N[σ0] : IT[σ][σ0][Id] }} by mauto 3.
+          assert {{ Δ0 ⊢s Id,,N[σ0] : Δ0, IT[σ][σ0]:Sort@s1 }} by mauto 4.
+          assert {{ Δ0 ⊢s σ∘σ0 : Γ }} by mauto 2.
+          assert {{ Δ0, IT[σ∘σ0]:Sort@s1 ⊢s q (σ∘σ0) : Γ, IT:Sort@s1 }} by mauto 4.
+          assert {{ Δ0 ⊢ IT[σ∘σ0] ≈ IT[σ][σ0] : Sort@s1 }} by mauto 3.
+          assert {{ ⊢ Δ0 }} by mauto 2.
+          assert {{ ⊢ Δ0, IT[σ][σ0]:Sort@s1 ≈ Δ0, IT[σ∘σ0]:Sort@s1 }} by mauto 4.
+          assert {{ Δ0 ⊢s Id,,N[σ0] : Δ0, IT[σ∘σ0]:Sort@s1 }} by mauto 4.
+          eapply wf_exp_eq_sub_compose_sort; mauto 2.
         }
+        
         eapply wf_exp_eq_conv' with (A:= {{{ OT[q (σ∘σ0)][(Id,,N[σ0])] }}}); mauto 3.
         eapply wf_exp_eq_app_cong'.
         -- specialize (H12 _ {{{σ ∘ σ0}}} _ ltac:(mauto 3) ltac:(eassumption)).
-           rewrite wf_exp_eq_sub_compose with (M := M) in H12; mauto 3.
+           rewrite wf_exp_eq_sub_compose_typ with (M := M) in H12; mauto 3.
            bulky_rewrite_in H12.
         -- assert (wf_typ_eq Δ0 {{{ IT[σ][σ0] }}} {{{ IT[σ∘σ0] }}}) by mauto.
            eapply wf_exp_eq_conv'; mauto 3.
         -- assert (wf_typ Δ0 {{{ IT[σ∘σ0] }}}) by mauto.
            assert (wf_typ Δ0 {{{ IT[σ][σ0] }}}) by mauto 4.
            econstructor; mauto 3.
-           transitivity {{{ IT[σ][σ0] }}}; mauto 3.        
+           
   - handle_functional_glu_sort_elem P.
     handle_per_sort_elem_irrel.
     pose proof H8.
@@ -279,7 +289,7 @@ Proof.
       specialize (H29 _ _ _ H19 H9).
       rewrite H5 in *.
       autorewrite with mcpts.
-      eassert (wf_exp Δ _ {{{ M[σ] }}}) by mauto 2.
+      eassert (wf_exp Δ _ {{{ M[σ] }}}) by mauto 3.
       autorewrite with mcpts in H30.
       rewrite @wf_exp_eq_pi_eta' with (M := {{{ M[σ] }}}); [| trivial].
       cbn [nf_to_exp].
@@ -289,13 +299,13 @@ Proof.
       simplify_evals.
       destruct (H2 _ ltac:(eassumption) _ ltac:(eassumption)) as [? []].
       specialize (H12 _ _ _ _ ltac:(trivial) (var_glu_elem_bot _ _ _ _ _ _ _ H H10)).
-      assert (IEL {{{ Δ,IT[σ] }}} {{{ IT[σ∘Wk] }}} {{{ #0 }}} d{{{ ⇑! a (length Δ) }}}).
+      assert (IEL {{{ Δ,IT[σ]:Sort@s1 }}} {{{ IT[σ∘Wk] }}} {{{ #0 }}} d{{{ ⇑! a (length Δ) }}}).
       {
         eapply glu_sort_elem_trm_resp_typ_exp_eq; mauto 3.
         symmetry.
         eapply exp_eq_sub_compose_typ_sort; mauto 4.
       }
-      specialize (H14 {{{Δ, IT[σ]}}} {{{σ ∘ Wk}}} _ _ ltac:(mauto) ltac:(eassumption) ltac:(eassumption)) as [? []].
+      specialize (H14 {{{Δ, IT[σ]:Sort@s1 }}} {{{σ ∘ Wk}}} _ _ ltac:(mauto) ltac:(eassumption) ltac:(eassumption)) as [? []].
       apply_equiv_left.
       destruct_rel_mod_app.
       simplify_evals.
@@ -305,20 +315,20 @@ Proof.
       do 2 (rewrite wf_exp_eq_sub_id in H41; mauto 4).
       etransitivity; [|eassumption].
       simpl.
-      assert (wf_exp {{{ Δ, IT[σ] }}} {{{ IT[σ∘Wk] }}} (@a_var P 0)).
+      assert (wf_exp {{{ Δ, IT[σ]:Sort@s1 }}} {{{ IT[σ∘Wk] }}} (@a_var P 0)).
       {
         eapply wf_conv' with (A := {{{ IT[σ][Wk] }}}); mauto 3.
-        symmetry; eapply wf_typ_eq_sub_compose; mauto 3.
+        symmetry; eapply wf_exp_eq_sub_compose_sort; mauto 3.
       }
       rewrite <- @sub_eq_q_sigma_id_extend; mauto 4.
-      assert (wf_typ {{{ Γ, IT }}} OT ) by mauto 3.
+      assert (wf_exp {{{ Γ, IT:Sort@s1 }}} {{{ Sort@s2 }}} OT ) by mauto 3.
       assert (wf_sub Δ Γ σ) by mauto 3.
-      assert (wf_sub {{{ Δ, IT[σ] }}} Δ {{{ Wk }}}) by mauto 3.
-      assert (wf_sub {{{ Δ, IT[σ] }}} Γ {{{ σ ∘ Wk }}}) by mauto 3.
-      assert (wf_sub {{{ Δ, IT[σ], IT[σ∘Wk] }}} {{{ Γ, IT }}} {{{ q (σ∘Wk ) }}}) by mauto 3.
-      assert (wf_exp {{{ Δ, IT[σ] }}} {{{ IT[σ∘Wk] }}} {{{ #0 }}}) by mauto 3.
-      assert (wf_sub {{{ Δ, IT[σ] }}} {{{ Δ, IT[σ], IT[σ∘Wk] }}} {{{ Id,,#0 }}}) by mauto 4.
-      assert (wf_typ_eq {{{ Δ, IT[σ] }}} {{{ OT[q (σ∘Wk)∘(Id,,#0)] }}} {{{ OT[q (σ∘Wk)][Id,,#0] }}}) by (symmetry; mauto 3).
+      assert (wf_sub {{{ Δ, IT[σ]:Sort@s1 }}} Δ {{{ Wk }}}) by mauto 3.
+      assert (wf_sub {{{ Δ, IT[σ]:Sort@s1 }}} Γ {{{ σ ∘ Wk }}}) by mauto 3.
+      assert (wf_sub {{{ Δ, IT[σ]:Sort@s1, IT[σ∘Wk]:Sort@s1 }}} {{{ Γ, IT:Sort@s1 }}} {{{ q (σ∘Wk ) }}}) by mauto 3.
+      assert (wf_exp {{{ Δ, IT[σ]:Sort@s1 }}} {{{ IT[σ∘Wk] }}} {{{ #0 }}}) by mauto 3.
+      assert (wf_sub {{{ Δ, IT[σ]:Sort@s1 }}} {{{ Δ, IT[σ]:Sort@s1, IT[σ∘Wk]:Sort@s1 }}} {{{ Id,,#0 }}}) by mauto 4.
+      assert (wf_exp_eq {{{ Δ, IT[σ]:Sort@s1 }}} {{{ Sort@s2 }}} {{{ OT[q (σ∘Wk)∘(Id,,#0)] }}} {{{ OT[q (σ∘Wk)][Id,,#0] }}}) by (symmetry; mauto 3).
       eapply wf_exp_eq_conv' with (A := {{{ OT[q (σ∘Wk)][Id,,#0] }}}); mauto 2.
       eapply wf_exp_eq_app_cong'; [| mauto 3].
       symmetry.
@@ -340,30 +350,6 @@ Proof.
       progressive_inversion.
       specialize (H3 (length Δ)) as [? []].
       firstorder.
-
-  - econstructor; eauto; intros.
-    progressive_inversion.
-    transitivity {{{ ℕ[σ] }}}; mauto 3.
-    econstructor; mauto 2.
-  - handle_functional_glu_sort_elem P.
-    match_by_head (@glu_sort_elem P) invert_glu_sort_elem.
-    apply_equiv_left.
-    repeat split; eauto.
-    econstructor; trivial.
-
-    intros.
-    saturate_weakening_escape.
-    assert {{ Δ ⊢ A[σ] ≈ ℕ[σ] : Sort@s }} by mauto 3.
-    assert {{ Δ ⊢ A[σ] ≈ ℕ[σ] }} by mauto 2.
-    rewrite <- wf_exp_eq_nat_sub; try eassumption.
-    mauto 3.
-  - econstructor; mauto 3.
-    + bulky_rewrite. mauto 3.
-    + apply_equiv_left. trivial.
-    + intros.
-      saturate_weakening_escape.
-      bulky_rewrite.
-      mauto using glu_nat_readback.
 Qed.
 
 
@@ -410,7 +396,7 @@ Hint Resolve realize_glu_typ_top realize_glu_elem_top : mcpts.
 Corollary var0_glu_elem {P} (pred_P : PredicativeSig P) : forall {s a typ_rel exp_rel Γ A},
     {{ DG a ∈ glu_sort_elem pred_P s ↘ typ_rel ↘ exp_rel }} ->
     {{ Γ ⊢ A ® typ_rel }} ->
-    {{ Γ, A ⊢ #0 : A[Wk] ® ⇑! a (length Γ) ∈ exp_rel }}.
+    {{ Γ, A:Sort@s ⊢ #0 : A[Wk] ® ⇑! a (length Γ) ∈ exp_rel }}.
 Proof.
   intros.
   eapply realize_glu_elem_bot; mauto 4.
