mechanization/theories/Core/Soundness/SubstitutionCases.v
@@ -5,18 +5,18 @@ From McPTS.Core.Semantic Require Import Realizability.
 From McPTS.Core.Soundness Require Import LogicalRelation TermStructureCases SortCases.
 Import Domain_Notations.
 
-Lemma presup_glu_rel_sub {P} (pred_P : PredicativeSig P) : forall {sts sts' Γ σ Δ},
-    {{ ⟪ pred_P ⟫ Γ : sts ⊩s σ : Δ : sts' }} ->
-    {{ ⟪ pred_P ⟫ ⊩ Γ : sts }} /\ {{ ⟪ pred_P ⟫ ⊩ Δ : sts' }}.
+Lemma presup_glu_rel_sub {P} (pred_P : PredicativeSig P) : forall {Γ σ Δ},
+    {{ ⟪ pred_P ⟫ Γ ⊩s σ : Δ }} ->
+    {{ ⟪ pred_P ⟫ ⊩ Γ }} /\ {{ ⟪ pred_P ⟫ ⊩ Δ }}.
 Proof.
   intros * [].
   destruct_conjs.
   split; eexists; eassumption.
 Qed.
 
-Lemma presup_left_glu_rel_sub {P} (pred_P : PredicativeSig P) : forall {sts sts' Γ σ Δ},
-    {{ ⟪ pred_P ⟫ Γ : sts ⊩s σ : Δ : sts' }} ->
-    {{ ⟪ pred_P ⟫ ⊩ Γ : sts }}.
+Lemma presup_left_glu_rel_sub {P} (pred_P : PredicativeSig P) : forall {Γ σ Δ},
+    {{ ⟪ pred_P ⟫ Γ ⊩s σ : Δ }} ->
+    {{ ⟪ pred_P ⟫ ⊩ Γ }}.
 Proof.
   intros * []%presup_glu_rel_sub.
   eassumption.
@@ -25,9 +25,9 @@ Qed.
 #[export]
 Hint Resolve presup_left_glu_rel_sub : mcpts.
 
-Lemma presup_right_glu_rel_sub {P} (pred_P : PredicativeSig P) : forall {sts sts' Γ σ Δ},
-    {{ ⟪ pred_P ⟫ Γ : sts ⊩s σ : Δ : sts' }} ->
-    {{ ⟪ pred_P ⟫ ⊩ Δ : sts' }}.
+Lemma presup_right_glu_rel_sub {P} (pred_P : PredicativeSig P) : forall {Γ σ Δ},
+    {{ ⟪ pred_P ⟫ Γ ⊩s σ : Δ }} ->
+    {{ ⟪ pred_P ⟫ ⊩ Δ }}.
 Proof.
   intros * []%presup_glu_rel_sub.
   eassumption.
@@ -36,9 +36,9 @@ Qed.
 #[export]
 Hint Resolve presup_right_glu_rel_sub : mcpts.
 
-Lemma glu_rel_sub_id {P} (pred_P : PredicativeSig P) : forall {sts Γ},
-    {{ ⟪ pred_P ⟫ ⊩ Γ : sts }} ->
-    {{ ⟪ pred_P ⟫ Γ : sts ⊩s Id : Γ : sts }}.
+Lemma glu_rel_sub_id {P} (pred_P : PredicativeSig P) : forall {Γ},
+    {{ ⟪ pred_P ⟫ ⊩ Γ }} ->
+    {{ ⟪ pred_P ⟫ Γ ⊩s Id : Γ }}.
 Proof.
   intros * [Sb].
   do 2 eexists; repeat split; mauto.
@@ -50,9 +50,9 @@ Qed.
 #[export]
 Hint Resolve glu_rel_sub_id : mcpts.
 
-Lemma glu_rel_sub_weaken {P} (pred_P : PredicativeSig P) : forall {Γ sts A s},
-    {{ ⟪ pred_P ⟫ ⊩ Γ, A : (s :: sts) }} ->
-    {{ ⟪ pred_P ⟫ Γ, A : (s :: sts) ⊩s Wk : Γ : sts }}.
+Lemma glu_rel_sub_weaken {P} (pred_P : PredicativeSig P) : forall {Γ A s},
+    {{ ⟪ pred_P ⟫ ⊩ Γ, A:Sort@s }} ->
+    {{ ⟪ pred_P ⟫ Γ, A:Sort@s ⊩s Wk : Γ }}.
 Proof.
   intros * [SbΓA].
   inversion_clear H.
@@ -67,10 +67,10 @@ Qed.
 #[export]
 Hint Resolve glu_rel_sub_weaken : mcpts.
 
-Lemma glu_rel_sub_compose {P} (pred_P : PredicativeSig P) : forall {sts1 sts2 sts3 Γ1 σ2 Γ2 σ1 Γ3},
-    {{ ⟪ pred_P ⟫ Γ1 : sts1 ⊩s σ2 : Γ2 : sts2 }} ->
-    {{ ⟪ pred_P ⟫ Γ2 : sts2 ⊩s σ1 : Γ3 : sts3 }} ->
-    {{ ⟪ pred_P ⟫ Γ1 : sts1 ⊩s σ1 ∘ σ2 : Γ3 : sts3 }}.
+Lemma glu_rel_sub_compose {P} (pred_P : PredicativeSig P) : forall {Γ1 σ2 Γ2 σ1 Γ3},
+    {{ ⟪ pred_P ⟫ Γ1 ⊩s σ2 : Γ2 }} ->
+    {{ ⟪ pred_P ⟫ Γ2 ⊩s σ1 : Γ3 }} ->
+    {{ ⟪ pred_P ⟫ Γ1 ⊩s σ1 ∘ σ2 : Γ3 }}.
 Proof.
   intros * Hσ2 Hσ1.
   assert {{ Γ2 ⊢s σ1 : Γ3 }} by mauto.
@@ -93,24 +93,28 @@ Qed.
 #[export]
 Hint Resolve glu_rel_sub_compose : mcpts.
 
-Lemma glu_rel_sub_extend {P} (pred_P : PredicativeSig P) (full_P : FullSig P) : forall {sts sts' Γ σ Δ M A s s'},
-    {{ ⟪ pred_P ⟫ Γ : sts ⊩s σ : Δ : sts' }} ->
-    {{ ⟪ pred_P ⟫ Δ : sts' ⊩ A : Sort@s : s' }} ->
-    {{ ⟪ pred_P ⟫ Γ : sts ⊩ M : A[σ] : s }} ->
-    {{ ⟪ pred_P ⟫ Γ : sts ⊩s (σ ,, M) : Δ , A : (s :: sts') }}.
+Lemma glu_rel_sub_extend {P} (pred_P : PredicativeSig P) (full_P : FullSig P) : forall {Γ σ Δ M A s s'},
+    {{ ⟪ pred_P ⟫ Γ ⊩s σ : Δ }} ->
+    {{ ⟪ pred_P ⟫ Δ ⊩ A : Sort@s > s' }} ->
+    {{ ⟪ pred_P ⟫ Γ ⊩ M : A[σ] > s }} ->
+    {{ ⟪ pred_P ⟫ Γ ⊩s (σ ,, M) : Δ , A:Sort@s }}.
 Proof.
   intros * Hσ HA HM.
   assert {{ Γ ⊢s σ : Δ }} by mauto 3.
   assert {{ Δ ⊢ A : Sort@s }} by mauto 3.
   assert {{ Γ ⊢ M : A[σ] }} by mauto 3.
   assert {{ Δ ⊢ Sort@s : Sort@s' }} by (eapply glu_rel_exp_typ_well_sorted; mauto 2).
-  assert (exists s'', {{ Δ ⊢ Sort@s'' ≈ Sort@s' }} /\ Ax P s s'') as [s'' []] by (eapply wf_exp_sort_sort; mauto 2).  
-  (* assert (exists s''', Ax P s'' s''') as [s'''] by (eapply full_P; mauto 2). *)
-  (* assert {{ ⟪ pred_P ⟫ Γ : sts ⊩ Sort@s : Sort@s'' : s''' }} by mauto 3. *)
-  (* assert {{ Γ ⊢ Sort@s[σ] ≈ Sort@s }} by mauto 3. *)
-  (* assert {{ ⟪ pred_P ⟫ Γ : sts ⊩ A[σ] : Sort@s : s' }} by mauto 3. *)
+  assert (Ax P s s') by (eapply glu_rel_exp_sort_implies_ax; mauto 2).
   destruct Hσ as [SbΓ [SbΔ]].
   destruct_conjs.
+
+  (* assert (exists s'', {{ Δ ⊢ Sort@s'' ≈ Sort@s' }} /\ Ax P s s'') as [s'' []] by (eapply wf_exp_sort_sort; mauto 2).   *)
+  (* (* assert (exists s''', Ax P s'' s''') as [s'''] by (eapply full_P; mauto 2). *) *)
+  (* (* assert {{ ⟪ pred_P ⟫ Γ : sts ⊩ Sort@s : Sort@s'' : s''' }} by mauto 3. *) *)
+  (* (* assert {{ Γ ⊢ Sort@s[σ] ≈ Sort@s }} by mauto 3. *) *)
+  (* (* assert {{ ⟪ pred_P ⟫ Γ : sts ⊩ A[σ] : Sort@s : s' }} by mauto 3. *) *)
+  (* destruct Hσ as [SbΓ [SbΔ]]. *)
+  (* destruct_conjs. *)
 
   destruct HA as [Sb []].
   destruct HM as [Sb' []].
@@ -121,16 +125,16 @@ Proof.
   do 2 eexists; repeat split; mauto.
   - econstructor; mauto 3; try reflexivity.
     intros.
-    rewrite <- H14 in H5.
+    rewrite <- H13 in H4.
     assert (glu_rel_exp_with_sub pred_P s' Δ0 A {{{ Sort@s }}} σ0 ρ) by mauto 2.
     mauto 2.
     
   - intros.
     handle_functional_glu_ctx_env P.
     destruct_glu_rel_sub_with_sub.
-    rewrite <- H14 in H8.
-    destruct_glu_rel_sub_with_sub.
-    rewrite <- H15 in H5.
+    rewrite <- H14 in H4.
+    (* destruct_glu_rel_exp_with_sub. *)
+    rewrite <- H13 in H11.
     (* rewrite <- H14 in H12. *)
     (* rewrite <- H14 in H16. *)
     destruct_glu_rel_exp_with_sub.
@@ -144,8 +148,8 @@ Proof.
     rename m into a.
     assert {{ Δ0 ⊢s σ0 : Γ }} by mauto 4.
     econstructor; mauto 3.
-    assert {{ Δ0 ⊢s (σ,,M)∘σ0 : Δ, A }} by mauto 3.
-    assert {{ Δ0 ⊢s (σ,,M)∘σ0 ≈ (σ∘σ0),,M[σ0] : Δ, A }} by mauto 3.
+    assert {{ Δ0 ⊢s (σ,,M)∘σ0 : Δ, A:Sort@s }} by mauto 3.
+    assert {{ Δ0 ⊢s (σ,,M)∘σ0 ≈ (σ∘σ0),,M[σ0] : Δ, A:Sort@s }} by mauto 3.
     assert {{ Δ0 ⊢s Wk∘((σ,,M)∘σ0) : Δ }} by mauto 4.
     assert {{ Δ0 ⊢s Wk∘((σ,,M)∘σ0) ≈ Wk∘((σ∘σ0),,M[σ0]) : Δ }} by mauto 4.
     assert {{ Δ0 ⊢ M[σ0] : A[σ][σ0] }} by mauto 3.
@@ -153,13 +157,13 @@ Proof.
     assert {{ Δ0 ⊢s Wk∘((σ∘σ0),,M[σ0]) ≈ σ∘σ0 : Δ }} by mauto 3.
     assert {{ Δ0 ⊢s Wk∘((σ,,M)∘σ0) ≈ σ∘σ0 : Δ }} by mauto 3.
     econstructor; mauto 4.
-    + assert {{ Δ, A ⊢s Wk : Δ }} by mauto 4.
+    + assert {{ Δ, A:Sort@s ⊢s Wk : Δ }} by mauto 4.
       assert {{ Δ0 ⊢ A[Wk][(σ,,M)∘σ0] ≈ A[Wk∘((σ,,M)∘σ0)] : Sort@s }} as -> by (symmetry; mauto 3).
       assert {{ Δ0 ⊢ A[Wk∘((σ,,M)∘σ0)] ≈ A[σ∘σ0] : Sort@s }} as -> by mauto 3.
       assert {{ Δ0 ⊢ A[σ∘σ0] ≈ A[σ][σ0] : Sort@s }} by mauto 3.
-      rewrite -> H29.
-      assert {{ Δ, A ⊢ #0 : A[Wk] }} by mauto 3.
-      assert {{ Δ0 ⊢ #0[(σ,,M)∘σ0] ≈ #0[(σ∘σ0),,M[σ0]] : A[Wk][(σ,,M)∘σ0] }} by mauto 3.
+      rewrite -> H30.
+      assert {{ Δ, A:Sort@s ⊢ #0 : A[Wk] }} by mauto 3.
+      assert {{ Δ0 ⊢ #0[(σ,,M)∘σ0] ≈ #0[(σ∘σ0),,M[σ0]] : A[Wk][(σ,,M)∘σ0] }} by mauto 4.
       assert {{ Δ0 ⊢ #0[(σ,,M)∘σ0] ≈ #0[(σ∘σ0),,M[σ0]] : A[σ][σ0] }} as -> by mauto 4.
       assert {{ Δ0 ⊢ #0[(σ∘σ0),,M[σ0]] ≈ M[σ0] : A[σ∘σ0] }} by mauto.
       assert {{ Δ0 ⊢ #0[(σ∘σ0),,M[σ0]] ≈ M[σ0] : A[σ][σ0] }} as -> by (eapply wf_exp_eq_conv; mauto 4).
@@ -172,4 +176,3 @@ Qed.
 
 #[export]
 Hint Resolve glu_rel_sub_extend : mcpts.
-
