mechanization/theories/Core/Soundness/TermStructureCases.v
@@ -5,9 +5,9 @@ From McPTS.Core.Semantic Require Import Realizability.
 From McPTS.Core.Soundness Require Import LogicalRelation.
 Import Domain_Notations.
 
-Lemma presup_glu_rel_exp {P} (pred_P : PredicativeSig P) (full_P : FullSig P) : forall {sts s Γ M A},
-    {{ ⟪ pred_P ⟫ Γ : sts ⊩ M : A : s }} ->
-    {{ ⟪ pred_P ⟫ ⊩ Γ : sts }} /\ (exists s', {{ ⟪ pred_P ⟫ Γ : sts ⊩ A : Sort@s : s' }}).
+Lemma presup_glu_rel_exp {P} (pred_P : PredicativeSig P) (full_P : FullSig P) : forall {s Γ M A},
+    {{ ⟪ pred_P ⟫ Γ ⊩ M : A > s }} ->
+    {{ ⟪ pred_P ⟫ ⊩ Γ }} /\ (exists s', {{ ⟪ pred_P ⟫ Γ ⊩ A : Sort@s > s' }}).
 Proof.
   intros * [? []].
   split; [eexists; eassumption |].
@@ -24,9 +24,9 @@ Proof.
   eapply glu_sort_elem_trm_typ; mauto 2.
 Qed.
 
-Lemma presup_ctx_glu_rel_exp {P} (pred_P : PredicativeSig P) (full_P : FullSig P) : forall {sts s Γ M A},
-    {{ ⟪ pred_P ⟫ Γ : sts ⊩ M : A : s }} ->
-    {{ ⟪ pred_P ⟫ ⊩ Γ : sts }}.
+Lemma presup_ctx_glu_rel_exp {P} (pred_P : PredicativeSig P) (full_P : FullSig P) : forall {s Γ M A},
+    {{ ⟪ pred_P ⟫ Γ ⊩ M : A > s }} ->
+    {{ ⟪ pred_P ⟫ ⊩ Γ }}.
 Proof.
   intros * []%presup_glu_rel_exp;
     eassumption.
@@ -35,9 +35,9 @@ Qed.
 #[export]
 Hint Resolve presup_ctx_glu_rel_exp : mcpts.
 
-Lemma presup_typ_glu_rel_exp {P} (pred_P : PredicativeSig P) (full_P : FullSig P) : forall {sts s Γ M A},
-    {{ ⟪ pred_P ⟫ Γ : sts ⊩ M : A : s }} ->
-    exists s', {{ ⟪ pred_P ⟫ Γ : sts ⊩ A : Sort@s : s' }}.
+Lemma presup_typ_glu_rel_exp {P} (pred_P : PredicativeSig P) (full_P : FullSig P) : forall {s Γ M A},
+    {{ ⟪ pred_P ⟫ Γ ⊩ M : A > s }} ->
+    exists s', {{ ⟪ pred_P ⟫ Γ ⊩ A : Sort@s > s' }}.
 Proof.
   intros * []%presup_glu_rel_exp;
     eassumption.
@@ -46,86 +46,69 @@ Qed.
 #[export]
 Hint Resolve presup_typ_glu_rel_exp : mcpts.
 
-Lemma glu_rel_exp_vlookup {P} (pred_P : PredicativeSig P) (full_P : FullSig P) : forall {sts Γ x A},
-    {{ #x : A ∈ Γ }} ->
-    {{ ⟪ pred_P ⟫ ⊩ Γ : sts }} ->
-    exists s,
-    {{ ⟪ pred_P ⟫ Γ : sts ⊩ #x : A : s}}.
+Lemma glu_rel_exp_vlookup {P} (pred_P : PredicativeSig P) (full_P : FullSig P) : forall {Γ x A s},
+    {{ #x : A : Sort@s ∈ Γ }} ->
+    {{ ⟪ pred_P ⟫ ⊩ Γ }} ->
+    {{ ⟪ pred_P ⟫ Γ ⊩ #x : A > s}}.
 Proof.
   intros * Hx.
-  gen sts.
-  induction Hx; intros * [Sb];
+  dependent induction Hx; intros * [Sb];
     match_by_head1 (@glu_ctx_env P) ltac:(fun H => invert_glu_ctx_env H).
   
   (* intros * [Sb] Hx. gen Sb. *)
   (* induction Hx; intros; *)
   (*   match_by_head1 (@glu_ctx_env P) ltac:(fun H => invert_glu_ctx_env H). *)
-  - exists s.
-    eexists.
+  - eexists.
     split; [econstructor |]; try reflexivity; mauto.
     intros.
     destruct_by_head (@cons_glu_sub_pred P).
     econstructor; mauto.
-  - assert (glu_ctx_env pred_P {{{ sts, s }}} Sb {{{ Γ, B }}}) by (econstructor; mauto).
-    assert (exists s, {{ ⟪ pred_P ⟫ Γ : sts ⊩ #n : A : s}}) as [s' Hn].
-    {
-      eapply IHHx.
-      econstructor; eauto.
-    }
-    assert (exists s, {{ Γ ⊢ A : Sort@s }}) as [s''] by (gen_presups; mauto 3).
-    inversion_clear Hn.
-    (* invert_glu_rel_exp Hn. *)
+  - assert (glu_ctx_env pred_P Sb {{{ Γ0, B:Sort@s0 }}}) by (econstructor; mauto).
+    specialize (IHHx pred_P full_P Γ0 A0 s ltac:(reflexivity) ltac:(reflexivity) ltac:(reflexivity) ltac:(econstructor; mauto 2)).
+    assert {{ Γ0 ⊢ A0 : Sort@s }} by mauto 3.
+    inversion_clear IHHx.
     destruct_conjs.
     handle_functional_glu_ctx_env P.
     do 2 eexists.
-    split.
     + econstructor; try reflexivity; mauto.
-   
-      (* intros. *)
-      (* dependent destruction H3. *)
-      (* handle_functional_glu_ctx_env P. *)
-      (* eapply H5. *)
-      (* eassumption. *)
-    + (* eexists. *)
-      intros.
+    + intros.
       destruct_by_head (@cons_glu_sub_pred P).
       rewrite <- H8 in H11.
       destruct_glu_rel_exp_with_sub.      
       simplify_evals.
       rename a into b.
       rename a0 into a.
-      assert {{ Dom a ≈ a ∈ per_sort pred_P s' }} as [] by mauto.      
+      assert {{ Dom a ≈ a ∈ per_sort pred_P s }} as [] by mauto.      
       eapply mk_glu_rel_exp_with_sub''; intuition mauto.      
       handle_functional_glu_sort_elem P.
       
-      assert {{ ⊢ Γ, B }} by mauto 3.
-      assert {{ Δ ⊢ A[Wk∘σ] : Sort@s' }} by (eapply glu_sort_elem_trm_sort_lvl; mauto 3).
-      assert {{ Δ ⊢ A[Wk][σ] ≈ A[Wk∘σ] : Sort@s' }} as ->.
+      assert {{ ⊢ Γ0, B:Sort@s0 }} by mauto 3.
+      assert {{ Δ ⊢ A0[Wk∘σ] : Sort@s }} by (eapply glu_sort_elem_trm_sort_lvl; mauto 3).
+      assert {{ Δ ⊢ A0[Wk][σ] ≈ A0[Wk∘σ] : Sort@s }} as -> by mauto 4.
+      assert {{ Γ0 ⊢ #n : A0 }} by mauto 4.
+      assert {{ Γ0, B:Sort@s0 ⊢ #n[Wk] : A0[Wk] }} by mauto 3.
+      assert {{ Γ0, B:Sort@s0 ⊢ #n[Wk] ≈ #(S n) : A0[Wk] }} by mauto 3.
+      assert {{ Δ ⊢ #n[Wk][σ] ≈ #(S n)[σ] : A0[Wk∘σ] }} as <-.
       {
-        assert (exists Δ0 K0, {{ Δ ⊢s Wk∘σ : Δ0 }} /\ {{ Δ0 ⊢ A : K0 }} /\ {{ Δ ⊢ K0[Wk∘σ] ≈ Sort@s' }}) as [Δ0 [K0 [? []]]] by mauto 2.
-        assert (exists Δ1, {{ Δ ⊢s σ : Δ1 }} /\ {{ Δ1 ⊢s Wk : Δ0 }}) as [Δ1 []] by mauto 2.
-        eapply wf_exp_eq_conv'; mauto 3.
-      }                                                                 
-      assert {{ Γ ⊢ #n : A }} by mauto 4.
-      assert {{ Γ, B ⊢ #n[Wk] : A[Wk] }} by mauto 3.
-      assert {{ Γ, B ⊢ #n[Wk] ≈ #(S n) : A[Wk] }} by mauto 3.
-      assert {{ Δ ⊢ #n[Wk][σ] ≈ #(S n)[σ] : A[Wk∘σ] }} as <- by (eapply wf_exp_eq_conv; mauto).
-      assert {{ Δ ⊢ #n[Wk∘σ] ≈ #n[Wk][σ] : A[Wk∘σ] }} as <- by mauto 3.
+        eapply wf_exp_eq_conv' with (A := {{{ A0[Wk][σ] }}}); mauto 3.
+        eapply wf_exp_eq_sub_cong_typ; mauto 3.
+      }
+      assert {{ Δ ⊢ #n[Wk∘σ] ≈ #n[Wk][σ] : A0[Wk∘σ] }} as <- by mauto 3.
       eassumption.
 Qed.
 
 #[export]
 Hint Resolve glu_rel_exp_vlookup : mcpts.
 
-Lemma glu_rel_exp_sub {P} (pred_P : PredicativeSig P) (full_P : FullSig P) : forall {sts Γ σ Δ sts' M A s},
-    {{ ⟪ pred_P ⟫ Γ : sts ⊩s σ : Δ : sts' }} ->
-    {{ ⟪ pred_P ⟫ Δ : sts' ⊩ M : A : s }} ->
-    {{ ⟪ pred_P ⟫ Γ : sts ⊩ M[σ] : A[σ] : s }}.
+Lemma glu_rel_exp_sub {P} (pred_P : PredicativeSig P) (full_P : FullSig P) : forall {Γ σ Δ M A s},
+    {{ ⟪ pred_P ⟫ Γ ⊩s σ : Δ }} ->
+    {{ ⟪ pred_P ⟫ Δ ⊩ M : A > s }} ->
+    {{ ⟪ pred_P ⟫ Γ ⊩ M[σ] : A[σ] > s }}.
 Proof .
   intros * Hσ HM.
   assert {{ Γ ⊢s σ : Δ }} by mauto 3.
   assert {{ Δ ⊢ M : A }} by mauto 3.
-  assert (exists s', {{ ⟪ pred_P ⟫ Δ : sts' ⊩ A : Sort@s : s' }}) as [s'] by mauto 3.
+  assert (exists s', {{ ⟪ pred_P ⟫ Δ ⊩ A : Sort@s > s' }}) as [s'] by mauto 3.
   destruct Hσ as [SbΓ [SbΔ]].
   destruct_conjs.
   inversion_clear HM as [? []].
@@ -149,10 +132,10 @@ Qed.
 Hint Resolve glu_rel_exp_sub : mcpts.
 
 
-Lemma glu_rel_exp_conv' {P} (pred_P : PredicativeSig P) (full_P : FullSig P) : forall {sts Γ M A A' s},
-    {{ ⟪ pred_P ⟫ Γ : sts ⊩ M : A : s }} ->
+Lemma glu_rel_exp_conv {P} (pred_P : PredicativeSig P) (full_P : FullSig P) : forall {Γ M A A' s},
+    {{ ⟪ pred_P ⟫ Γ ⊩ M : A > s }} ->
     {{ Γ ⊢ A ≈ A' : Sort@s }} ->
-    {{ ⟪ pred_P ⟫ Γ : sts ⊩ M : A' : s }}.
+    {{ ⟪ pred_P ⟫ Γ ⊩ M : A' > s }}.
 Proof.
   intros * [Sb [?]] HAA'.
   assert {{ ⟪ pred_P ⟫ Γ ⊨u A ≈ A' : Sort@s }} as [env_relΓ [? ?]] by (eapply completeness_fundamental_exp_eq; mauto 2).
@@ -207,88 +190,29 @@ Proof.
   eassumption.  
 Qed.
 
+#[export]
+Hint Resolve glu_rel_exp_conv : mcpts.
+ 
 
+Lemma glu_rel_exp_conv_sort {P} (pred_P : PredicativeSig P) (full_P : FullSig P) : forall {Γ M A s s'},
+    {{ ⟪ pred_P ⟫ Γ ⊩ M : A > s }} ->
+    {{ ⟪ pred_P ⟫ Γ ⊩ A > s' }} ->
+    {{ ⟪ pred_P ⟫ Γ ⊩ M : A > s' }}.
+Proof.
+  intros * [SbΓ []] [SbΓ' []].
+  handle_functional_glu_ctx_env P.
+  eexists; split; mauto 2.
+  intros.
+  assert (SbΓ' Δ σ ρ) by (eapply H4; eassumption).
+  destruct_glu_rel_exp_with_sub.
+  destruct_glu_rel_typ_with_sub.
+  simplify_evals.
+  econstructor; mauto 3.
 
-(* Lemma glu_rel_exp_conv {P} (pred_P : PredicativeSig P) (full_P : FullSig P) : forall {sts Γ M A A' s}, *)
-(*     {{ ⟪ pred_P ⟫ Γ : sts ⊩ M : A : s }} -> *)
-(*     {{ Γ ⊢ A ≈ A' }} -> *)
-(*     {{ ⟪ pred_P ⟫ Γ : sts ⊩ M : A' : s }}. *)
-(* Proof. *)
-(*   intros * [Sb [?]] HAA'. *)
-(*   assert {{ ⟪ pred_P ⟫ Γ ⊨ A ≈ A' }} as [env_relΓ [? ?]] by (eapply completeness_fundamental_typ_eq; mauto 2). *)
-  
-(*   assert (exists ρ ρ', initial_env Γ ρ /\ initial_env Γ ρ' /\ {{ Dom ρ ≈ ρ' ∈ env_relΓ }}) as [ρ [ρ']] by (eauto using per_ctx_then_per_env_initial_env). *)
-(*   destruct_conjs. *)
-(*   assert (exists elem_rel : relation (domain P), *)
-(*              rel_typ_unsorted pred_P A ρ A' ρ' elem_rel) as [elem_rel] by mauto. *)
-  
-  
-(*   destruct_by_head (@rel_typ_unsorted P). *)
-(*   simplify_evals. *)
-  
-(*   assert {{ Γ ⊢s Id ® ρ ∈ Sb }} by (eapply initial_env_glu_rel_exp; mauto 2). *)
-(*   destruct_glu_rel_exp_with_sub. *)
-(*   simplify_evals. *)
-  
-(*   eexists; split; [eauto |]. *)
-(*   intros. *)
-(*   assert (glu_rel_exp_with_sub pred_P s Δ M A σ ρ0) by mauto 2. *)
-(*   destruct H14. *)
-(*   simplify_evals. *)
-(*   handle_functional_glu_sort_elem P. *)
+  assert (per_sort pred_P s a a) by mauto 3.
+  eapply (glu_sort_elem_exp_conv pred_P H9 H7 H10); mauto 2.
+Qed.
 
-(*   assert (env_relΓ ρ0 ρ0) by (eapply glu_ctx_env_per_env; mauto 2). *)
-(*   assert (exists elem_rel0, rel_typ_unsorted pred_P A ρ0 A' ρ0 elem_rel0) as [elem_rel0] by mauto 2. *)
-(*   destruct_by_head (@rel_typ_unsorted P). *)
-(*   simplify_evals. *)
-(*   assert (per_typ_elem pred_P (per_sort pred_P s) d{{{ Sort@s }}} d{{{ Sort@s }}}) by (eapply per_typ_sort; reflexivity). *)
-(*   handle_per_typ_elem_irrel. *)
-(*   assert (per_sort pred_P s a0 a0) as [R] by mauto 3. *)
-(*   assert (per_sort_elem pred_P s elem_rel0 a0 a'0) by mauto 3. *)
-(*   assert (per_sort_elem pred_P s elem_rel0 a'0 a'0) by (transitivity a0; [symmetry |]; mauto 2). *)
-  
-(*   eapply mk_glu_rel_exp_with_sub''; mauto 3. *)
-(*   intros. *)
-(*   assert {{ Δ ⊢ A[σ] ≈ A'[σ] : Sort@s }} as <- by admit. *)
-
-(*   assert (glu_sort_elem pred_P s typ_rel1 exp_rel1 a0). *)
-(*   { *)
-(*     symmetry in H23. *)
-(*     eapply glu_sort_elem_resp_per_sort; mauto 3. *)
-(*   } *)
-(*   eapply glu_sort_elem_exp_conv with (a := a0) (a' := a0) (exp_rel := exp_rel0); mauto. *)
-
-(*   assert (typ_rel0 Δ {{{ A [σ] }}}) by (eapply glu_sort_elem_trm_typ; mauto 2). *)
-(*   handle_functional_glu_sort_elem P. *)
-(*   eassumption.   *)
-(* Qed. *)
-
-
-  
-(* Lemma glu_rel_exp_conv {P} (pred_P : PredicativeSig P) (full_P : FullSig P) : forall {sts s Γ M A A' }, *)
-(*     {{ ⟪ pred_P ⟫ Γ : sts ⊩ M : A : s }} -> *)
-(*     {{ Γ ⊢ A ≈ A' }} -> *)
-(*     {{ ⟪ pred_P ⟫ Γ : sts ⊩ M : A' : s }}. *)
-(* Proof. *)
-(*   intros. *)
-(*   enough {{ Γ ⊢ A ≈ A' : Sort@s }} by (eapply glu_rel_exp_conv'; mauto). *)
-(*   destruct H as [Sb [?]]. *)
-  
-(*   assert {{ ⟪ pred_P ⟫ Γ ⊨ A ≈ A' }} as [env_relΓ [? ?]] by (eapply completeness_fundamental_typ_eq; mauto 2).   *)
-(*   assert (exists ρ ρ', initial_env Γ ρ /\ initial_env Γ ρ' /\ {{ Dom ρ ≈ ρ' ∈ env_relΓ }}) as [ρ [ρ']] by (eauto using per_ctx_then_per_env_initial_env). *)
-(*   destruct_conjs. *)
-(*   assert (exists elem_rel : relation (domain P), rel_typ_unsorted pred_P A ρ A' ρ' elem_rel) by mauto 2. *)
-(*   destruct_conjs. *)
-(*   destruct_rel_typ_unsorted. *)
-  
-(*   assert {{ Γ ⊢s Id ® ρ ∈ Sb }} by (eapply initial_env_glu_rel_exp; mauto 2). *)
-(*   destruct_glu_rel_exp_with_sub. *)
-(*   simplify_evals. *)
-(*   assert (per_sort pred_P s a a) as [R] by mauto 2. *)
-(*   assert (per_sort_elem pred_P s H7 a a') by mauto 3. *)
-(*   assert (glu_sort_elem pred_P s typ_rel exp_rel a') by (eapply glu_sort_elem_resp_per_sort_elem with (typ_rel := typ_rel) (exp_rel := exp_rel); mauto 3). *)
-
-(*   assert {{ Γ ⊢ A[Id] ≈ A : Sort@s }} by mauto 4. *)
-(*   assert {{ Γ ⊢ A : Sort@s }} by mauto 3. *)
-  
-  
+#[export]
+Hint Resolve glu_rel_exp_conv_sort : mcpts.
+                                         
